---
title: Applications of Derivative Practice #2
author: Chris Agrella
date: 10/27/2021
output: pdf_document
---

## q1

- a) (-1, 1.5)U(2, 5)
- b) (-5, -1)U(1.5, 2)
- c) (-3, 0.5)
- d) (0.5, 5)
- e) x=-1 is a local minimum, x=1.5 is relative max, x=2 local min.
- f) x = 0.5 from concave up to concave down

## q2

- a) (-6, -2)U(0, 5)
- b) (-2, 0)
- c) (-6, -3)U(-1, 1)
- d) (-3, -1)U(1, 5)
- e) x=-2, maximum, x=0, minimum
- f) x=-3, x=-1, x=1

## q3

- \(f(x) = 3x^4 + 4x^3 - 6x^2\)
- \(f'(x) = 12x^3 + 12x^2 - 12x\)
  - \(0 = 12x^3 + 12x^2 - 12x\)
  - \(0 = 12x(x^2 + x - 1)\)
  - \(x = 0, x = \frac{-1 + \sqrt{5}}{2}, x = \frac{-1 - \sqrt{5}}{2}\)
- \(f''(x) = 36x^2 + 24x - 12\)
  - \(f''(0) < 0\)
  - \(f''(\frac{-1 + \sqrt{5}}{2}) > 0\)
  - \(f''(\frac{-1 - \sqrt{5}}{2}) > 0\)
  - \(f(\frac{-1 + \sqrt{5}}{2}) > f(\frac{-1 - \sqrt{5}}{2})\)
- Local Maximum is \(x = 0\)
- Local Minimum is \(x = \frac{-1 - \sqrt{5}}{2}\)
- \(f''(x) = 0\)v
  - \(36x^2 + 24x - 12 = 0\)
  - \(3x^2 + 2x - 1 = 0\)
  - \((x + 1)(x - \frac{1}{3})\)
  - \(x = -1, x = \frac{1}{3}\)
  - \(f''(-1 + 0.1) < 0, f''(-1 - 0.1) > 0\)
  - \(f''(\frac{1}{3} + \frac{1}{3}) > 0, f''(\frac{1}{3} - \frac{1}{3}) < 0\)
- Concave up from \((-\infty, -1)\cup (\frac{1}{3}, \infty)\)
- Concave down from \((-1, \frac{1}{3})\)
