---
title: Homework - Graded Assignment 01
author: Chris Agrella
date: 09/13/2021
output: pdf_document
---

## Question 1

1. Function must exist at \(f(x)\)
  
    - \(f(2) = k(2)^2 = 4k\)

2. \(\lim\limits_{x \rightarrow 2} f(x)\) must exist.
    - \(\lim\limits_{x \rightarrow 2^-} f(x) = kx^2\)
      - Plug in 2, \(\lim\limits_{x \rightarrow 2^-} f(x) = 4k\)
    - \(\lim\limits_{x \rightarrow 2^+} f(x) = 2x + k\)
      - Plug in 2, \(\lim\limits_{x \rightarrow 2^+} f(x) = k + 4\)
    - To ensure that the limits equal, we have to find the value of `k` that makes both sides of the limit exists
    - \(4k = k + 4\), \(4k - k = 4\), \(k - \frac{k}{4} = 1\), \(\frac{4k}{4} - \frac{k}{4} = 1\), \(\frac{3k}{4} = 1\), \(k = \frac{4}{3}\)
    - Plug in `k`to both forms.
      - \(\lim\limits_{x \rightarrow 2^-} f(x) = k(4)\), \(\lim\limits_{x \rightarrow 2^-} f(x) = \frac{16}{3}\)
      - \(\lim\limits_{x \rightarrow 2^+} f(x) = k(2)^2 = k(4) = 16/3\)
    - \(\lim\limits_{x \rightarrow 2} f(x) = \frac{16}{3}\)

3. Ensure that the value of the limit matches the value of the function.
    - For \(x = 2\), \(f(x) = kx^2\)
    - \(f(x) = \frac{4}{3}x^2\)
    - \(f(2) = \frac{4}{3}(2^2) = \frac{4}{3}(4) = \frac{16}{3}\)
    - \(f(x) = \lim\limits_{x \rightarrow 2}\)

Function is continuous at \(x = 2\) when \(k = \frac{4}{3}\).

## Question 2

### 2.a

![graph-a](https://i.imgur.com/6RBXfcR.png)

See Graph-A for table of values.

\(\lim\limits_{x \rightarrow 2} \frac{sin(2x)}{x} = 2\)

### 2.b

![graph-b](https://i.imgur.com/Xl8Mjad.png)

See Graph-B for table of values

Table shows \(\lim\limits_{x \rightarrow 0} \frac{sin(3x)}{x} = 3\)

## Question 3

- \(f(x) = x^2 - 2x + 2\)

### 3.a

- Form One
  - \(f'(a) = \lim\limits_{h \rightarrow 0} \frac{f(a+h) - f(a)}{h}\)
  - \(f'(2) = \lim\limits_{h \rightarrow 0} \frac{f(2+h) - f(2)}{h}\)
  - \(f'(2) = \lim\limits_{h \rightarrow 0} \frac{((2+h)^2 - 2(2+h) + 2) - ((2)^2 - 2(2) + 2)}{h}\)
  - \(f'(2) = \lim\limits_{h \rightarrow 0} \frac{((2+h)^2 - (4+2h) + 2) - (2)}{h}\)
    - \((2+h)^2 = (h + 2)(h + 2) = h^2 + 4h + 4\)
  - \(f'(2) =\lim\limits_{h \rightarrow 0} \frac{(h^2 + 4h + 4) - (4 + 2h) - 2}{h} \)
  - \(f'(2) =\lim\limits_{h \rightarrow 0} \frac{h^2 + 2h - 2}{h} \)
  - \(f'(2) =\lim\limits_{h \rightarrow 0} h + 2 - \frac{h}{2} \)
  - \(f'(2) =\lim\limits_{h \rightarrow 0} f(a) = (0) + 2 - \frac{0}{2} \)
  - \(f'(2) =\lim\limits_{h \rightarrow 0} f(a) = 2 \)

- Form Two
  - \(f'(a) = \lim\limits_{x \rightarrow a} \frac{f(x) - f(a)}{x - a}\)
  - \(f'(2) = \lim\limits_{x \rightarrow a} \frac{(x^2 - 2x + 2) - (2)}{x - 2}\)
  - \(f'(2) = \lim\limits_{x \rightarrow a} \frac{x^2 - 2x}{x - 2}\)
  - \(f'(2) = \lim\limits_{x \rightarrow a} \frac{x(x - 2)}{x - 2}\)
  - \(f'(2) = \lim\limits_{x \rightarrow a} (2) = 2\)
  - \(f'(2) = \lim\limits_{x \rightarrow a} f(x) = 2\)

### 3.b

- \(f'(x) =  \lim\limits_{h \rightarrow 0} \frac{f(x+h) - f(x)}{h}\)
- \(f'(x) = \lim\limits_{h \rightarrow 0} \frac{((x+h)^2 - 2(x+h) + 2) - (x^2 - 2x + 2)}{h}\)
  - \((x+h)^2 = (x+h)(x+h) = x^2 + 2hx + h^2\)
- \(f'(x) = \lim\limits_{h \rightarrow 0} \frac{(x^2 + 2hx + h^2 - 2x - 2h + 2) - x^2 +2x - 2}{h}\)
- \(f'(x) = \lim\limits_{h \rightarrow 0} \frac{2hx + h^2 - 2h }{h}\)
- \(f'(x) = \lim\limits_{h \rightarrow 0} 2x + h - 2 +\frac{-4}{h}\)
- \(f'(x) = \lim\limits_{h \rightarrow 0} 2x + (0) - 2 +\frac{-4x + 4}{(0)}\)
- \(f'(x) = 2x - 2\)

### 3.c

![graph-c](https://i.imgur.com/DsKitaO.png)

See Graph-C

I plotted the two functions onto Desmos on the same coordinate plane.

## Question 4

![graph-d](https://i.imgur.com/oHrCx8J.png)

See Graph-D

I used a piecewise function to create a hole in the graph, and then showed the points where the function's values were.