---
title: Calc Homework
author: Chris Agrella
date: 09/23/2021
output: pdf_document
---

## pg 297

### q221

- \(f(x) = (3x^2 + 1)^3\)
- \(u = 3x^2 + 1\), \(y = x^3\)
- \(f'(x) = 3u^2 * 6x\)
- \(f'(x) = 18x(3x^2 + 1)^2\)

### q222

- \(f(x) = \sin^5(x) = (\sin(x))^5\)
- \(u = \sin(x)\), \(y = u^5\)
- \(f'(x) = 5u^4 * \cos(x)\)
- \(f'(x) = 5(\sin(x))^4 * \cos(x)\)

### q223

- \(f(x) = (\frac{x}{7} + \frac{7}{x})^7\)
- \(u = (\frac{x}{7} + \frac{7}{x})\), \(y = u^7\)
- \(f'(x) = 7u^6 * (\frac{1}{7} - 7x^{-2})\)
- \(f'(x) = 7(\frac{x}{7} + \frac{7}{x})^6 * (\frac{1}{7} - 7x^{-2})\)

### q230

- \(f(x) = (\cos(\pi x))^3\)
- \(y = v^3\), \(v = \cos(u)\), \(u = \pi x\)
- \(f'(x) = 3v^2 * -\sin(u) * \pi\)
- \(f'(x) = 3(\cos(\pi x))^2 * -\sin(\pi x) * \pi\)

### q231

- \(f(x) = (2x^3 - x^2 + 6x + 1)^3\)
- \(y = u^3\), \(u = 2x^3 - x^2 + 6x + 1\)
- \(f'(x) = 3u^2 * (6x^2 - 2x + 6)\)
- \(f'(x) = 3(2x^3 - x^2 + 6x + 1)^2 * (6x^2 - 2x + 6)\)

### q233

- \(f(x) = (\tan x + \sin x)^{-3}\)
- \(u = \tan x + \sin x\), \(y = u^{-3}\)
- \(f'(x) = -3u^{-4} * (\sec^2x + \cos x)\)
- \(f'(x) = -3(\tan x + \sin x)^{-4} * (\sec^2x + \cos x)\)

### q234

- \(f(x) = x^2(\cos x)^4\)
  - \(u = \cos x\), \(y = u^4\)
  - \(4u^3 * -\sin x\)
- \(f'(x) = (2x)((\cos x)^4) + (x^2)(4(\cos x)^3 * -\sin x)\)

### q235

- \(f(x) = \sin(\cos 7x))\)
- \(u = 7x\), \(v = \cos u\), \(y = \sin v\)
- \(f'(x) = \cos(\cos(7x)) * -\sin(7x) * 7\)

### q241

- \(f(x) = -\sin(\frac{x}{2})\)
- \(u = \frac{x}{2}\), \(y = -\sin(x)\)
- \(f'(x) = -\cos(\frac{x}{2}) * \frac{1}{2}\)
- \(y - y_1 = m(x - x_1)\)
  - \(x_1 = 0\), \(y_1 = f(0) = 0\)
  - \(m = f'(0) = -\frac{1}{2}\)
- \(y = -\frac{1}{2}x\)

![tangent-one](https://i.imgur.com/IYzLchP.png)

### q242

- \(f(x) = (3x + \frac{1}{x})^2\)
  - \(u = 3x + x^{-1}\), \(y = u^2\)
- \(f'(x) = 2u * (3 - x^{-2})\)
- \(f'(x) = 2(3x + \frac{1}{x}) * (3 - x^{-2})\)
- \(f'(x) = (6x + \frac{2}{x}) * (3 + \frac{1}{-x^2})\)
- \(f'(1) = m = 16\)
- \(y = 16x\)

## pg 298

### q245

- \(h(x) = f(g(x))\)
  - \(u = g(x)\), \(y = f(x)\)
- \(h'(x) = f'(g(x)) * g'(x)\)
- \(h'(0) = f'(g(0)) * g'(0)\)
- \(h'(0) = 5 * 2\)
- \(h'(0) = 10\)

### q248

- \(h(x) = (\frac{f(x)}{g(x)})^2\)
  - \(u = \frac{f(x)}{g(x)}\), \(y = v^2\)
- \(h'(x) = 2v * \frac{f'(x)g(x)-f(x)g'(x)}{(g(x))^2}\)
- \(h'(x) = 2(\frac{f(x)}{g(x)}) * \frac{f'(x)g(x)-f(x)g'(x)}{(g(x))^2}\)
- \(h'(3) = 2(\frac{3}{2}) * \frac{(-3)(2) - (3)(3)}{(3)^2}\)
- \(h'(3) = 3 * \frac{15}{9} = \frac{45}{9} = 5\)

### q254

- \(s(t) = -3\cos(\pi t + \frac{\pi}{4})\)
  - \(u = \pi t + \frac{\pi}{4}\), \(v = -3 \cos (u)\)
- \(s'(t) = 3 \sin (u) * \pi\)
- \(s'(t) = 3 \sin (\pi t + \frac{\pi}{4}) * \pi\)
- \(s(1.5) = -2.121 = 2.121\) inches downwards
- \(s'(1.5) = -6.66\) in/s downward
