---
title: Calc Homework - Derivative Practice 6
author: Chris Agrella
date: 09/26/2021
output: pdf_document
---

## Q1

### a)

- \(f(x) = -4*(3x^2-2x+1)^{-3}\)
  - \(u = 3x^2 - 2x + 1\), \(y = -4x^{-3}\)
- \(f'(x) = 12u^{-4} * (6x - 2)\)
- \(f'(x) = 12(3x^2 - 2x + 1)^{-4} * (6x - 2)\)

### b)

- \(f(x) = (\cos{3\sqrt{x}})^2\)
  - \(u = 3(x^{1/2})\), \(v = \cos{u}\), \(y = v^2\)
- \(f'(x) = (2v)(-\sin(u))*3(\frac{1}{2}x^{-1/2})\)
- \(f'(x) = 2(\cos(3\sqrt{x}))(-\sin(3\sqrt{x}))*3(\frac{1}{2}x^{-1/2})\)

### c)

- \(f(x) = \frac{x^2 + 1}{\sqrt{x}}\)
  - \(a' = 2x\), \(b' = \frac{1}{2}x^{-1/2}\)
- \(f'(x) = \frac{(2x)(\sqrt{x})-(x^2 + 1)(\frac{1}{2}x^{-1/2})}{x}\)

### d)

- \(f(x) = \sqrt{sin(x^7)}\)
  - \(u = x^7\), \(v = \sin(u)\), \(y = \sqrt{v}\)
- \(f'(x) = \frac{1}{2}(v)^{-1/2} * \cos(u) * 7x^6\)
- \(f'(x) = \frac{1}{2}(\sin(x^7))^{-1/2} * \cos(x^7) * 7x^6\)

### e

- \(f(x) = \sqrt{x}(\tan(x^3))^4\)
  - \(u = x^3\), \(v = \tan(u)\), \(y = v^4\)
  - \(4v^3 * (\sec(u))^2\ * 3x^2\)
  - \(4(\tan(x^3)) * (\sec(x^3))^2 * 3x^2\)
- \((\frac{1}{2}x^{-1/2})((\tan(x^3))^4) + (\sqrt{x})(4(\tan(x^3)) * (\sec(x^3))^2 * 3x^2)\)

### f

- \(f(x) = (5x + 8)^7(1 - x^{1/3})\)
  - \(u = 5x + 8\), \(v = u^7\)
  - \(7u^6*5\)
  - \(35(5x+8)^6\)
  - \((1 - x^{1/3})' = -\frac{1}{3x^{2/3}}\)
- \(f'(x) = (35(5x+8)^6)(1 - x^{1/3}) + ((5x + 8)^7)(\frac{-1}{3x^{2/3}})\)

### g

- \(f(x) = (\frac{x-5}{2x+1})^5\)
  - \(u = \frac{x-5}{2x+1}\), \(y = x^5\)
  - \(u'= \frac{(1)(2x+1) - (x-5)(2)}{(2x + 1)^2}\)
- \(f'(x) = 5u^4 * (\frac{(1)(2x+1) - (x-5)(2)}{(2x + 1)^2})\)
- \(f'(x) = 5(\frac{x-5}{2x+1})^4* \frac{(2x+1) - (x-5)(2)}{(2x + 1)^2}\)

## q2

- \(f(x) = x^2(5 - x^2)^{1/2}\)
  - \(u = 5 - x^2\), \(y = u^{1/2}\)
  - \(\frac{1}{2}(5 - x^2)^{-1/2} * -2x\)
- \(f'(x) = (2x)(5-x^2)^{1/2} + (x^2)(\frac{1}{2}(5 - x^2)^{-1/2} * -2x)\)
- \(m = f'(1) = 3.5\)
- \(x_1 = 1, y_1 = f(1) = 2\)
- \(y - 2 = 3.5(x - 1)\)

## q3

### 3.a)

- False, because that does not match the chain rule, for the chain rule you would do \(f'(u) * g'(x)\)

### 3.b)

- False, because you would have to multiply by \(g'(x)\) to satisfy the chain rule.
