---
title: Homework
author: Chris Agrella
date: 08/25/2021
output: pdf_document

---

Limits
======

Question 5
----------

\(\lim\limits_{x\rightarrow0} \dfrac{\sqrt{x+1}-1}{x}\)

\(\dfrac{\sqrt{x+1}-1}{x} * \dfrac{\sqrt{x+1}+1}{\sqrt{x+1}+1}\) - Multiply by cognate of square root.

\(\dfrac{x}{x(\sqrt(x+1)+1)}\) - Don't distribute!

\(\dfrac{1}{\sqrt{x+1}+1}\) - Cancel out the \(x\)

Plug in 0, \(\dfrac{1}{1+1}\), \(\frac{1}{2}\)

__\(\lim\limits_{x\rightarrow0} \dfrac{\sqrt{x+1}-1}{x} = \frac{1}{2}\)__

Question 6 (in class)
---------------------
\(\lim\limits_{h\rightarrow0} \frac{(1+h)^2-1}{h}\)

\(\frac{h^2+2h+1-1}{h}\)

\(\frac{(h^2+2h)}{h}\)

\(\frac{(h+2)(h)}{h}\)

\(\frac{h+2}{1}\)

\(\lim\limits_{h\rightarrow0} \frac{(1+h)^2-1}{h} = 2\)

Textbook Questions
==================

Question 30
-----------
|x|f(x)|
|-|----|
|0.9|-1.9|
|0.99|-1.99|
|0.999|-1.999|
|0.9999|-1.9999|
|1.1|2.1|
|1.01|2.01|
|1.001|2.001|
|1.0001|2.0001|

\(\lim\limits_{x \rightarrow 1^+} f(x) = 2 \neq \lim\limits_{x \rightarrow 1^-} f(x) = -2\)

Question 35
-----------
|x|\(\frac{sin(2x)}{x}\)|
|-|----|
|-0.1|1.9867|
|-0.01|1.9999|
|-0.001|1.9999|
|-0.0001|2|
|0.1|1.9867|
|0.01|1.9999|
|0.001|1.9999|
|0.0001|2|

\(\lim\limits_{x \rightarrow 0} \frac{sin(2x)}{x} = 2\)

Question 38
-----------

|x|f(x)|
|-|----|
|0.9|0.7436|
|0.99|0.7494|
|0.999|0.7499|
|0.9999|0.7499|
|1.1|0.7561|
|1.01|0.7506|
|1.001|0.7501|
|1.0001|0.7500|

\(\frac{x^2-4}{x^2+x-6}\)

\(\frac{(x+2)(x-2)}{(x-2)(x+3)}\)

\(\frac{x+2}{x+3}\)

\(\frac{(1)+2}{(1)+3}\)

\(\frac{3}{4}\)

\(\lim\limits_{x \rightarrow 1} f(x) = \frac{3}{4}\)

Question 47
-----------

\(\lim\limits_{x\rightarrow-2^+} f(x) = 3\) is False, because the limit approaching from the right goes to \(\infty\) (is unbounded), not 3.

Question 49
-----------

\(\lim\limits_{x\rightarrow6} f(x) = 5\) is False, because the limit does not approach the same number (\(5\)) from both sides of the limit.


Question 103
------------

\(\lim\limits_{x \rightarrow -2^-} \frac{2x^2 + 7x - 4}{x^2 + x - 2}\)

\(\frac{(x+4)(2x-1)}{(x+2)(x-1)}\)

__\(\lim\limits_{x \rightarrow -2^-} \frac{2x^2 + 7x - 4}{x^2 + x - 2} \rightarrow \infty\) (unbounded)__
