---
title: Homework
author: Chris Agrella
date: 10/06/2021
output: pdf_document
---

## q302

- \(x^2y = y - 7\)
- \(x^2(y) - (y) + 7 = 0\)
- \((2x)(y) + (x^2)\frac{dy}{dx} - 1\frac{dy}{dx}\)
- \(\frac{dy}{dx}(x^2 -1 ) = -2xy\)
- \(\frac{dy}{dx} = \frac{-2xy}{x^2 - 1}\)

## q306

- \(-xy - 2 = \frac{x}{7}\)
- \(-xy - 2 = \frac{1}{7}x\)
- \(\frac{d}{dx}(-xy - 2) = \frac{d}{dx}(\frac{1}{7}(x))\)
- \(-(\frac{d}{dx}(xy)) = \frac{d}{dx}(\frac{x}{7})\)
- \(-x\frac{dy}{dx} + y = \frac{1}{7}\)
- \(-x\frac{dy}{dx} = \frac{1}{7} - y\)
- \(\frac{dy}{dx} = -\frac{1}{7x} - \frac{y}{x}\)

## q309

- \(x^3y + xy^3 = 8\)
- \((3x^2)(y) + (x^3)(\frac{dy}{dx}) + (1)(y^3)+(x)(3y^2)\frac{dy}{dx}\)
- \(\frac{dy}{dx}(x^3 + 3xy^2) = -3x^2y+y^3\)
- \(\frac{dy}{dx} = -\frac{3x^2y + y^3}{x^3 + 3xy^2}\)

## q311

- \(x^2y^2 + 5xy = 14\)
- \(((2x)(y^2) + (x^2)(2y)\frac{dy}{dx}) + 5(y + x\frac{dy}{dx})\)
- \(\frac{dy}{dx}(2x^2y + 5x) = -2xy^2 + 5y\)
- \(\frac{dy}{dx} = -\frac{2xy^2 + 5y}{2x^2y + 5x}\)
- \(-\frac{2(2)(1)^2 + 5(1)}{2(2)^2(1) + 5(2)}\)
- \(-\frac{4 + 5}{8 + 10}\)
- \(-\frac{9}{18}\)
- \(m = -\frac{1}{2}\)
- \(y - 1 = -\frac{1}{2}(x - 2)\)

## q314

- \(\frac{x}{y} + 5x - 7 = -\frac{3}{4}y\)
- \(\frac{x'y - xy'}{y^2} + 5 = -\frac{3}{4}\frac{dy}{dx}\)
- \(\frac{y - x\frac{dy}{dx}}{y^2}= -\frac{3}{4}\frac{dy}{dx} - 5\)
- \(y - x\frac{dy}{dx} = (-\frac{3}{4}\frac{dy}{dx} - 5)y^2\)
- \(y - x\frac{dy}{dx}\ = -\frac{3y^2}{4}\frac{dy}{dx} - 5y^2\)
- \(y + 5y^2 = \frac{dy}{dx}(x - \frac{3y^2}{4})\)
- \(\frac{dy}{dx} = \frac{y + 5y^2}{x - \frac{3y^2}{4}}\)
- \(m = -11\)
- \(y - 2 = -11(x - 1)\)

## q325

- \(85 = \frac{1}{3}\pi(x^2y)\)
- \(0 = \frac{\pi}{3}(2xy + x^2y')\)
- \(\frac{\pi}{3} (-x^2)\frac{dy}{dx} = \frac{\pi}{3}2xy\)
- \(\frac{dy}{dx} = \frac{2xy}{-x^2}\)
