---
title: Graded Assignment #3
author: Chris Agrella
date: 10/27/2021
output: pdf_document
---

## q1

- \(f(x) = e^{-kx}\sqrt{x}\)
- \(f'(x) = (e^{-kx})(\frac{1}{2}x^{-1/2}) + (e^{-kx})(-k)(\sqrt{x})\)
  - \(f'(x) = (e^{-kx})(\frac{1}{2}x^{-1/2}) + -ke^{-kx}\sqrt{x}\)
- \(f'(x) = \frac{1}{2}x^{-1/2}e^{-kx} - ke^{-kx}\sqrt{x}\)
  - \(f'(x) = 0\)
  - \(0 = \frac{1}{2}x^{-1/2}e^{-kx} - ke^{-kx}x^{1/2}\)
  - \(0 = (e^{-kx})(\frac{1}{2}x^{-1/2} - kx^{1/2})\)
  - \(0 = (x^{-1/2} - 2kx^{1/2})\)
  - \(x = \frac{1}{2k}\)
