---
title: Graded Practice 02
author: Chris Agrella
date: 10/05/2021
output: pdf_document
---

## q1

### 1.a)

- \(f(x) = \sin(\sqrt{3x + 1})\)
  - \(u = 3x + 1\), \(v = \sqrt{x}\), \(y = \sin(x)\)
- \(f'(x) = \cos(\sqrt{3x + 1})(\frac{1}{2}(3x + 1)^{-1/2})(3)\)

### 1.b)

- \(f(x) = e^{x^2 + 7}\)
  - \(u = x^2 + 7\), \(v = e^x\)
- \(f'(x) = (e^u)(2x)\)
- \(f'(x) = e^{x^2+7}(2x)\)

### 1.c)

- \(f(x) = \sqrt{e^{4x}*\cos(-\frac{1}{2}x)}\)
  - \(u = e^{4x}*\cos(-\frac{1}{2}x)\), \(v = \sqrt{u}\)
  - \(u' = (4e^{4x})(\cos(-\frac{1}{2}x))+(e^{4x})(\sin(-\frac{1}{2}x)(\frac{1}{2}))\)
- \(f'(x) = \frac{1}{2}(e^{4x}*\cos(-\frac{1}{2}x))^{-1/2}*((4e^{4x})(\cos(-\frac{1}{2}x))+(e^{4x})(\sin(-\frac{1}{2}x)(\frac{1}{2})))\)

### 1.d)

- \(f(x) = \ln((\tan(x+1))^2)\)
- \(f(x) = 2\ln(\tan(x+1))\)
  - \(u = x + 1\), \(v = \tan(x)\), \(y = 2\ln(x)\)
- \(f'(x) = \frac{2}{\tan(x+1)}*(sec(x+1)^2)\)

## q2

- \(f(x) = x\ln(x)\)
- \(f'(x) = 1(\ln(x)) + (x)(\frac{1}{x})\)
- \(f'(x) = \ln(x) + 1\)
  - \(x_1 = 2\), \(y_1 = f(2) = 1.39\), \(m = f'(2) = 1.69\)
- \(y - 1.39 = 1.69(x - 2)\)

## q3

- \(f(x) = \frac{x}{x^2 + 1}\)
- \(f(x) = x(x^2 + 1)^{-1}\)
  - \(u = x^2 + 1\), \(v = x^{-1}\)
  - inner derivative \(-(x^2 + 1)^{-2} * 2x\)
- \(f'(x) = 1(x^2+1)^{-1} + (x)(-2x(x^2 + 1)^{-2})\)
  - \(x_1 = 2\), \(y_1 = f(2) = 0.4\), \(m = f'(2) = -0.12\)
- \(y - 0.4 = -0.12(x - 2)\)

## q4

- \(x^3 + y^3 = 3xy\)
- \(x^3 + (y)^3 - 3xy = 0\)
- \(3x^2 + (3y^2)\frac{dy}{dx} + 3y - 3(\frac{dy}{dx}) = 0\)
- \(\frac{dy}{dx}(3y^2 - 3) = -3x^2 - 3y\)
- \(\frac{dy}{dx} = \frac{-3x^2 - 3y}{3y^2 - 3}\)
- \(\frac{dy}{dx} = \frac{x^2 - y}{x - y^2}\)
  - \(m = -1\)
- \(y - \frac{3}{2} = -(x - \frac{3}{2})\)