---
title: Mean Value Theorem HW
author: Chris Agrella
date: 10/11/2021
output: pdf_document
---

## q1

### a

- \(m = \frac{f(4) - f(-2)}{4 - (-2)} = \frac{0 + 6}{6} = 1\)
- \(x_1 = -2, y_1 = -6\)
- \(y + 6 = (x + 2)\)
- \(y = x - 4\)

### b

- \(m_{sec} = 1\), \(f(x) = x^2 - x - 12\), \(f'(x) = 2x - 1\)
- \(f'(c) = \frac{f(4) - f(-2)}{4 + 2} = 1\)
  - \(f'(x) = 2x - 1\)
  - \(1 = 2x - 1\)
  - \(2x = 2\)
  - \(x = 1\)
- \(x = 1\) is where they are equal.

### c

- \(f(1) = 1^2 - 1 - 12 = -12\)
- \(f'(1) = 2(1) - 1 = 1\)
- \(x_1 = 1, y_1 = -12, m = 1\)
- \(y + 12 = (x - 1)\)
