# Calc Notes 9/30

## Implicit Differentiation Exercises

### 1.a)

- \(x^2 - y^3 = 0\)
- \(2x - 3y^2 = 0\)
- \(-3y^2 = -2x\)
- \(\frac{-3y^2}{-3y^2} = \frac{-2x}{-3y^2}\)
- \(f'(x) = \frac{2x}{3y^2}\)

### 1.b)

- \(4x^2 + 9y^2 = 36\)
- \(8x + 18y = 0\)
- \(18y = - 8x\)
- \(f'(x) = \frac{-8x}{18y}\)

### 1.c)

- \(\cos(y) + \sqrt{x} = 5\)
- \(-\sin(y)(\frac{d}{dx}y) + \frac{1}{2}x^{-1/2} = 0\)
- \(\frac{d}{dx}[y] = \frac{\frac{1}{2}x^{-1/2}}{-\sin(y)}\)
  - \(\frac{1}{2\sqrt{x}} * \frac{\sqrt{x}}{\sqrt{x}}\)
  - \(\frac{\sqrt{x}}{2x}\)
- \(f'(x) = \frac{\sqrt{x}}{2x\sin(y)}\)

### 1.d)

- \(x^2 + y^2 + 3x - 5y = 25\)
- \(2x + 2(y)(\frac{d}{dx}) + 3 - 5(y)^0(\frac{d}{dx}) = 0\)
- \((y)^2\frac{dy}{dx} - 5(y)\frac{dy}{dx} = -2x - 3\)
- \(\frac{dy}{dx}(2y - 5) = -2x - 3\)
- \(f'(x) = \frac{-2x - 3}{2y - 5}\)

> With \(y^1\), it becomes \(1\)

### 1.e)

- \(x^2 + xy - y^2\)
- \(\frac{d}{dx}(x^2) + \frac{dy}{dx}(xy) - \frac{dy}{dx}(y^2) = 0\)
- \(2x + \frac{d}{dx}[x](y) + (x)(\frac{d}{dx}[f(x)]) - 2y(\frac{dy}{dx})\)
- \(2x + 1(y) + x(\frac{dy}{dx}) - 2y(\frac{dy}{dx}) = 0\)
- \(\frac{dy}{dx}(x - 2y) = -2x - y\)
- \(\frac{dy}{dx} = \frac{-2x - y}{x - 2y}\)

### 1.f)

- \(x^3 + 2xy + y^2 = 4\)
- \(3x^2 + (\frac{d}{dx}(2x)*y + 2x\frac{dy}{dx}) + 2y\frac{dy}{dx} = 0\)
- \(3x^2 + 2y + 2x(\frac{dy}{dx}) + 2y\frac{dy}{dx} = 0\)
- \(\frac{dy}{dx} = \frac{-3x^2 - 2y}{2x + 2y}\)

### 2)

- \(x^2 + xy + y^2 = 3\)
- \(2x + y + \frac{dy}{dx}x + 2y\frac{dy}{dx} = 0\)
- \(\frac{dy}{dx} = \frac{-2x - y}{x + 2y}\)
- \(\frac{-2(1) - 1}{1 + 2}\)
- \(\frac{-3}{3} = -1 = m\)
- \(y - 1 = -(x - 1)\)
- \(y = -x + 2\)

### 3)

- \(y + x^2y^3 = 10\)
- \(1\frac{dy}{dx} + (2x)(y^3) + (x^2)(3y^2\frac{dy}{dx}) = 0\)
- \(2x(y^3) + (x^2)(3y^2\frac{dy}{dx}) + \frac{dy}{dx}(1) = 0\)
- \(x^2(3y^2)(\frac{dy}{dx}) + \frac{dy}{dx}(1) = - 2x(y^3)\)
- \(\frac{dy}{dx} = \frac{-2x(y^3)}{1 + x^2(3y^2)}\)
