---
title: Notes
author: Chris Agrella
date: 09/08/2021
output: pdf_document
---

## Expanding

- Expanding a binomial \((A + B)^2\) gives \(A^2 + 2AB + B^2\)

- Expanding a trinomial \((A + B)^3\) gives \(A^3 + 3A^2B + 3AB^2 + B^3\)

## Wrapping up limits

\(\lim\limits_{x\rightarrow2} f(x) = 1\), \(\lim\limits_{x\rightarrow 4^-} f(x) = 3\), \(\lim\limits_{x \rightarrow 4^+} f(x) = 6\), \(x = 4\) is undefined

![limit-graph](https://i.imgur.com/X2K6JKT.png)

## Derivative Forms

1. \(\lim\limits_{h \rightarrow 0} \frac{f(a+h)-f(a)}{h}\)
2. \(\lim\limits_{h \rightarrow a} \frac{f(x) - a}{x - a}\)
3. \(\lim\limits_{h \rightarrow 0} \frac{f(x+h) - f(x)}{h}\) - to find the derivative function.
    - Another form \(\lim\limits_{\Delta x \rightarrow 0} \frac{f(x + \Delta x) - f(x)}{\Delta x}\)
    - Represents the \(\Delta x\) approaching the instantaneous rate of change.

Tangent line is \(y = m(x - a) + f(a)\)

## Power Rule of Differentiation

- \(f(x) = x^2, f'(x) = 2x\)
- \(f(x) = x^3, f'(x) = 3x^2\)
- \(f(x) = x^4, f'(x) = 4x^3\)
- **.
\(f(x) = x^n, f'(x) = nx^{n-1}\)**
