---
title: Calc Notes
author: Chris Agrella
date: 09/22/2021
output: pdf_document
---

## Homework Review

1. q1

- a. \(f'(x)\) does not exist since the limit approaches different values from both sides.
- b. Limit of function approaches infinity, and therefore does not exist

> Vertical Tangent Line, and vertical lines have undefined slope.

- c. Approaches infinity and therefore does not exist

- All functions are continuous but not differentiable.

## Notes

- Derivative is increasing when it is > 0, and vice versa.

## Exercises

1. q1
    - a. y - 2.6 = 0.4(x - 10)
    - b. 3
2. q2: for hw

## Algebra Review

1. multiplying functions
    - a. \(f(g(x)) = 3(5x^2 + x + 2)-1\)
    - b. \(g(f(x)) = 5(3x - 1)^2 + (3x - 1) + 2\)
2. reverse composition
    - a. \(f(x) = 3x^5\), \(g(x) = x^2 - 4x + 1\)
    - b. \(f(x) = \cos x\), \(g(x) = x^3\)
    - c. \(f(x) = x^2\), \(g(x) = \tan x\)

## Derivative Practice

1. \(f(x) = \sin(2x)\)
    - \(f'(x) = \frac{d}{dx}[\sin x] * \frac{d}{dx}[2x]\)
    - \(f'(x) = \cos x * 2 = 2\cos 2x\)
2. \(f(x) = \tan(-2x)\)
    - \(f'(x) = \frac{dy}{du} * \frac{du}{dx}\)
    - \(f'(x) = \sec^2(u) * -2\)
    - \(f'(x) = \frac{d}{dx}[\tan (-2x)] * \frac{d}{dx}[-2x]\)
    - \(f'(x) = \sec^2(-2x) * -2\)
    - \(f'(x) = -2\sec^2(-2x)\)
3. \(f(x) = \sqrt{3x}\)
    - \(f'(x) = \frac{dy}{du} * \frac{du}{dx}\)
    - \(f'(x) = (\frac{1}{2}(3x)^{-1/2})* 3\)
    - \(f'(x) = \frac{3}{2}(3x)^{-1/2}\)
4. \(f(x) = \sqrt{6x + 5} - 11\)
    - \(u = 6x + 5\)
    - \(y = x^{1/2} - 11\)
    - \(f'(x) = \frac{dy}{du} * \frac{du}{dx}\)
    - \(f'(x) = \frac{1}{2}u^{-1/2} * 6\)
    - \(f'(x) = 3u^{-1/2}\)
    - \(f'(x) = 3(6x+5)^{-1/2}\)
5. \(f(x) = (x^2 + 1)^{20}\)
    - \(u = x^2 + 1\), \(y = x^{20}\)
    - \(f'(x) = \frac{dy}{du} * \frac{du}{dx}\)
    - \(f'(x) = 20u^{19} * 2x\)
    - \(f'(x) = 20(x^2 + 1)^{19} * 2x\)
6. \(f(x) = (5x^2 - 3x + 1)^{10}\)
    - \(u = 5x^2 - 3x + 1\), \(y = x^{10}\)
    - \(10u^9 * (10x - 3)\)
    - \(f'(x) = 10(5x^2 - 3x + 1)^9 * (10x - 3)\)
7. \(f(x) = e^{4x}\)
    - \(u = e^x\), \(y = x^4\)
    - \(f'(x) = 4u^3 * e^x\)
    - \(f'(x) = 4(e^x)^4\), \(f'(x) = 4e^{4x}\)
8. \(f(x) = tan(3x + \frac{\pi}{2})\)
    - \(u = 3x + \frac{\pi}{2}\), \(y = \tan x\)
    - \(f'(x) = \sec^2u * 3\)
    - \(f'(x) = 3\sec^2(3x + \frac{\pi}{2})\)
9. \(f(x) = \cos(3x^2)\)
    - \(u = 3x^2\), \(y = \cos x\)
    - \(f'(x) = -\sin (u) * 6x\)
    - \(f'(x) = -6x\sin(3x^2)\)
10. \(f(x) = \sin^4(x^2+1)\)
    - \(f(x) = (\sin(x^2 + 1))^4\)
    - \(y = v^4\)
    - \(v = \sin u\), \(u = x^2 + 1\)
    - Take the derivative of each part
    - \(f'(x) = 2x * \cos(u) * 4u^3\)
    - Replace the other variables
    - \(f'(x) = 2x * \cos(x^2 + 1) * 4(\sin(x^2 + 1))^3\)
    - Start with outer-most function and work inside.
11. \(f(x) = \frac{1}{(-x + 9)^5}\)
    - \(u = -x + 9\), \(y = x^{-5}\)
    - \(f'(x) = -5u^{-6} * (-1)\)
    - \(f'(x) = \frac{5}{(9 - x)^6}\)
