---
title: Notes
author: Chris Agrella
date: 09/09/2021
output: pdf_document
---

## Derivative Notation

If finding the derivate of \(y = 4\), you can write the derivate as \(\frac{dy}{dx}\), and plugging in 4 gives us \(\frac{d[4]}{dx}\)

### Example

- Find Derivate of \(y = 3x^0\)

- Power rule gives us \(\frac{dy}{dx} 0 * 3x^{0-1} = \frac{dy}{dx} = 0\)

## Example of a constant

- \(y = \pi\)
- \(\frac{dy}{dx} = 0\), since a constant's derivative is always 0.

## Example using a function (sum rule)

- \(y = x^2 + x + 1\)
  - Can use the sum rule to take the derivative of each term
  - \(\frac{dy}{dx} (x^2) + \frac{dy}{dx} (x) + \frac{dy}{dx} (1)\)
    - Using the power rule to convert \(x^2\) to \(2x\)
  - \(\frac{dy}{dx} = 2x + 1 + 0\)
  - \(\frac{dy}{dx} = 2x + 1\)
  - "The derivative of the sum is equal to the sums of the derivatives."
    - Also works with subtraction!

## Example using Constant Multiple rule

- The derivative of a constant multiplied by a function is the same as the constant multiplied by the derivative.

- \(y = 2 * x^2\)
- \(\frac{dy}{dx} = \frac{d[2x^2]}{dy} = 2\frac{d[x^2]}{dy}\)
- \(2 *\frac{d[x^2]}{dy}=2* 2x\)
- \(\frac{dy}{dx} = 4x\) or \(y' = 4x\)

Another Example of Constant Multiple:

- \(y = 4x^2\)
- \(y' = 2 *(4x^{2-1}) = 2* 4x = 8x\)
- \(y' = 8x\)

## Required Knowledge

- Using the Power Rule
  - Using algebra to re-write terms
  - Use sum-difference property of derivatives to isolate terms.
  - Use the constant-multiple property of derivatives to isolate functions.

## Example Problems

### q 109

- \(f(x) = 8x^4 + 9x^2 - 1\)
- \(f'(x) = \frac{dy}{dx}(8x^4) + \frac{dy}{dx}(9x^2) + \frac{dy}{dx}(-1)\)
- \(f'(x) = 8\frac{dy}{dx}(x^4) + 9\frac{dy}{dx}(x^2) + \frac{dy}{dx}(-1)\)
- \(f'(x) = 8(4x^3) + 9(2x) + 0\)
- \(f'(x) = 32x^3 + 18x\)

### q 110

- \(f(x) = x^4 + \frac{2}{x}\)
- \(f(x) = x^4 + 2x^{-1}\)
- \(f'(x) = \frac{dy}{dx}(x^4) + 2\frac{dy}{dx}(x^{-1})\)
- \(f'(x) = 4x^3 + 2(-x^{-2})\)
- \(f'(x) = 4x^3 + -2x^{-2}\)

### q 112

- \(f(x) = (x + 2)(2x^2 - 3)\)
- \(f(x) = (2x^3 - 3x)+(4x^2 - 6) = 2x^3 + 4x^2 - 3x + - 6\)
- \(f'(x) = 2\frac{dy}{dx}(x^3) + 4\frac{dy}{dx}(x^2) - 3\frac{dy}{dx}x + \frac{dy}{dx}(6)\)
- \(f'(x) = 2(3x^2) + 4(2x) + 3(-1)\)
- \(f'(x) = 6x^2 + 8x - 3\)

### q 113

- \(f(x) = x^2(\frac{2}{x^2} + \frac{5}{x^3})\)
- \(f(x) = 2 + \frac{5}{x}\)
- \(f(x) = 2 + 5x^{-1}\)
- \(f'(x) = \frac{dy}{dx} (2) + 5\frac{dy}{dx}(x^{-1})\)
- \(f'(x) = 0 + 5(-x^{-2})\)
- \(f'(x) = -5x^{-2} = \frac{-5}{x^2}\)

### q 114

- \(f(x) = \frac{x^3 + 2x^2 - 4}{3}\)
- \(f(x) = \frac{1}{3}x^3 + \frac{1}{3}2x^2 - \frac{4}{3}\)
- \(f'(x) = \frac{1}{3}\frac{dy}{dx}(x^3) + \frac{2}{3}\frac{dy}{dx}(x^2) - \frac{1}{3}\frac{dy}{dx}4\)
- \(f'(x) = \frac{1}{3}(2x^2) + \frac{1}{3}(2x) + 0\)
- \(f'(x) = \frac{2x^2 + 2x}{3}\)

### q 115

- \(f(x) = \frac{4x^3 - 2x + 1}{x^2}\)
- \(f(x) = \frac{4x^3}{x^2} - \frac{2x}{x^2} + \frac{1}{x^2}\)
- \(f(x) = 4x - \frac{2}{x} + \frac{1}{x^2}\)
- \(f(x) = 4x - 2x^{-1} + x^{-2}\)
- \(f'(x) = 4\frac{dy}{dx}(x) - 2\frac{dy}{dx}(x^{-1}) + \frac{dy}{dx}(x^{-2})\)
- \(f'(x) = 4(1) - 2(-x^{-2}) + (-2x^{-3})\)
- \(f'(x) = 4 + 2x^{-2} - 2x^{-3} = 4 + \frac{2}{x^2} - \frac{2}{x^3}\)
